\documentclass{article}
\usepackage{amsmath}
\title{Tutorial for Week 9 - Answers}
\author{Ben Weston}
\date{\today}

\begin{document}
\maketitle
\begin{enumerate}\setcounter{enumi}{1}
        \item{
                        \begin{enumerate}
                                \item $S=(P\wedge Q\wedge R)\vee(P\wedge\neg Q\wedge R)\vee(P\wedge\neg Q\wedge\neg R)$ where $S$ is the output of the circuit. Therefore, $S=0$.
                                \item As above the DNF is: $(P\wedge Q\wedge R)\vee(P\wedge\neg Q\wedge R)\vee(P\wedge\neg Q\wedge\neg R)$
                                \item{        \begin{align*}
                                                        S &= (P\wedge Q\wedge R)\vee(P\wedge\neg Q\wedge R)\vee(P\wedge\neg Q\wedge\neg R)\\
                                                          &= (P\wedge((Q\wedge R)\vee(\neg Q\wedge R)\vee(\neg Q\wedge\neg R)))\\
                                                          &= (P\wedge((Q\wedge R)\vee(\neg Q\wedge(R\vee\neg R))))\\
                                                          &= (P\wedge((Q\wedge R)\vee(\neg Q \wedge 1)))\\
                                                          &= (P\wedge((Q\wedge R)\vee \neg Q))\\
                                                          &= (P\wedge((\neg Q\vee Q)\wedge(\neg Q\vee R)))\\
                                                          &= (P\wedge(1\wedge(\neg Q\vee R)))\\
                                                          &= (P\wedge(\neg Q\vee R))
                                                \end{align*}
                                        }
                        \end{enumerate}
                }
\end{enumerate}

\end{document}
