---
title: COMP109 - Strong Induction
tags: COMP109 Lectures
---
For a normal case of mathematical induction you can prove that a statement holds for all numbers from a particular start point. 

It uses a base case so show that it holds for an individual number and an induction rule that proves that it holds for all numbers following.

* Prove that the property holds for the natural number &#92;(n=0&#92;)
* Prove that if the property holds for &#92;(n=0,1,\ldots,m&#92;) (and not just for m) then it holds for &#92;(n=m+1&#92;).

Can also be used to prove a property for all integers greater than or equal to some particular natural number &#92;(b&#92;).

## Example 1
Every natural number &#92;(n \geq 2&#92;), is a prime or product of primes.

### Base Case
Take &#92;(n=2&#92;)

Then &#92;(n&#92;) is a prime number.

### Inductive Step
Assume that the property holds for &#92;(n=m&#92;) so every number &#92;(i&#92;) such that &#92;(2\leq i\leq m&#92;) is a prime or a product of primes. 

Now consider &#92;(n=m+1&#92;).

We proceed by considering cases.

#### Case 1
&#92;(m+1&#92;) is prime.

There is nothing to prove.

#### Case 2
&#92;(m+1&#92;) is not prime.

So &#92;(m+1=k\times l&#92;), where &#92;(k\neq1,\ k\neq m+1&#92;) and &#92;(l\neq 1,\ l\neq\ m+1&#92;)

So &#92;(k\geq2,\ l\geq2,\ k\leq m,\ l \leq m&#92;)

So &#92;(k=P&#95;1\ldots P&#95;n,\ l=Q&#95;1\ldots Q&#95;m&#92;). Then &#92;(k\times l&#92;) is a product of primes.

## Example 2
For any integer &#92;(n\geq1&#92;), if &#92;(x&#95;1,x&#95;2,\ldots,x&#95;n&#92;) are &#92;(n&#92;) numbers, then no matter how the parentheses are inserted into their product, the number of multiplications used to compute the products is &#92;(n-1&#92;).

As the number are all individual you can't use tricks like using already computed values to speed up the computation.
{:.info}

### Base Case
&#92;[
X&#95;1 \text{ for } n=1,\ n-1=0
&#92;]

### Induction Step
Suppose that no matter how I put parentheses on a sequence of &#92;(i&#92;) elements, where &#92;(1\leq i\leq m&#92;), I need &#92;(m-1&#92;) multiplications. 

Consider, where &#92;(1\leq l \leq m&#92;):
&#92;[
\underbrace{\underbrace{(x&#95;1\times\ldots)}&#95;{l}\times\underbrace{(\ldots\times x&#95;{m+1})}&#95;{m+1-l}}&#95;{m+1}
&#92;]

By induction hypothesis
&#92;[\require{cancel}\cancel{l}-1+m+1-\cancel{l}-\cancel{1}+\cancel{1}=(m+1)-1&#92;]

This proves that the property holds for the next value to infinitude. &#92;(\square&#92;)
