---
title: COMP109 - Mathematical Induction
tags: COMP109 Lectures
---
* They are used to check conjectures about outcomes of processes that occur repeatedly and according to definite patterns.
* In general, mathematical induction is a method for proving that a property defined for integers $$n$$ is true for all values of $$n$$ that are greater than or equal to come initial integer.

## Generic Particular v.s. Induction for Universal Statements
### Generalisation from the generic particular:

"Suppose that $$x$$ is a particular but arbitrarily chosen..." "...property holds for this $$x$$..." "...then the property holds for all $$x$$"
{:.info}

This argument states that as we have chosen an arbitrary value from a set then the argument will hold for all numbers within the same set.

## Induction
We apply a process to all the values in a set. This process is carried on until an arbitrary value is reached.

* Prove that the property holds for some initial value (e.g. $$n=0$$).
* Prove that if the property hold for $$n=m$$ (for any natural number $$m$$) then it holds for $$n=m+1$$.

### Example
For a set of dominoes the following process can be applied:

For a domino at position $$i$$, when it is pushed the domino at position $$i+1$$ will fall sequentially.

The conclusion can be that all of the dominoes will fall.

### Typical Structure
We prove the statement by mathematical induction on $$n$$.

#### Base Case
Show that the property hold for some initial value (e.g. $$n=0$$).

#### Inductive Step
Assume that the property holds for $$n=m$$. Show that is hold for $$n=m+1$$.

#### Conclusion
You can now conclude that the property holds for every natural number $$n$$.

### Carl Friedrich Gauss
$$1+\ldots+100=5050$$

If you split the number line in the middle the sum of every column is 101. With 50 columns the answer is 5050.

For every natural number $$n$$, 
$$0+1+\ldots+n=\frac{n(n+1)}{2}$$

#### Proof
##### Base Case
$$n=0$$ 

$$0 = \frac{0(0+1)}{2} = 0$$

##### Inductive Step
Suppose that for $$n=m$$ the property holds.

Then $$0+1+\ldots+m=\frac{m(m+1)}{2}$$

Consider the statement for $$n=m+1$$.

$$0+1+2+\ldots+m+(m+1)$$.

By induction hypothesis, $$0+1+\ldots+m=\frac{m(m+1)}{2}$$

So, $$0+1+\ldots+m+(m+1)=\frac{m(m+1)}{2}+(m+1)$$

$$=\frac{m(m+1)}{2}+\frac{2(m+1)}{2}=\frac{m(m+1)+2(m+1)}{2}$$

$$=\frac{(m+1)(m+2)}{2}=\frac{(m+1)((m+1)+1)}{2}=\frac{n(n+1)}{2}$$

This shows that for any sequential number the fraction simplifies to the statement, thus proving that it holds for any number.
