---
title: COMP109 - Logic - 4
tags: COMP109 Lectures
---
## Digital Logic Circuits
### In Series
This circuit produces similar results to an AND gate:

![series]({site.baseurl}/assets/COMP109/Lectures/2020-12-03-1-1.svg)

## In Parallel
This circuit produces similar results to an OR gate:

![parallel]({site.baseurl}/assets/COMP109/Lectures/2020-12-03-1-2.svg)

Modern computers use **logic gates**.

## Basic Logic Gates
### AND Gate

![and]({site.baseurl}/assets/COMP109/Lectures/2020-12-03-1-3.svg)

| &#92;(P&#92;) | &#92;(Q&#92;) | &#92;(R&#92;) |
| :-: | :-: | :-: |
| 1 | 1 | 1 |
| 1 | 0 | 0 |
| 0 | 1 | 0 | 
| 0 | 0 | 0 |

### OR Gate

![or]({site.baseurl}/assets/COMP109/Lectures/2020-12-03-1-4.svg)

| &#92;(P&#92;) | &#92;(Q&#92;) | &#92;(R&#92;) |
| :-: | :-: | :-: |
| 1 | 1 | 1 |
| 1 | 0 | 1 |
| 0 | 1 | 1 | 
| 0 | 0 | 0 |

### NOT Gate

![not]({site.baseurl}/assets/COMP109/Lectures/2020-12-03-1-5.svg)

| &#92;(P&#92;) | &#92;(R&#92;) |
| :-: | :-: |
| 1 | 0 |
| 0 | 1 |

### Rules for a Combinatorial Circuit

* Never combine two input wires.
* A single input wire can be split partway and used as input for two separate gates.
* An output wire can be used as input.
* No output of a gate can eventually feed back into that gate.

There are some additional examples in [the video](https://liverpool.instructure.com/courses/27539/modules/items/317194) that I haven't covered here as they are very logical.
{:.info}

### Multi-Input Gates
If you want to and together mutiple values you can either use a multi-input package or string together a multi-gate package. Here are two equivalent diagrams:

![multi-in]({site.baseurl}/assets/COMP109/Lectures/2020-12-03-1-6.svg)

![multi-gate]({site.baseurl}/assets/COMP109/Lectures/2020-12-03-1-7.svg)

## Designing a Circuit for a Given Input/Output Table

Say you have the following table of inputs and outputs you want to have in a circuit:

| Input | Input | Input | Output |
| :-: | :-: | :-: | :-: |
| P | Q | R | S |
| 1 | 1 | 1 | 1 |
| 1 | 1 | 0 | 1 |
| 1 | 0 | 1 | 1 |
| 1 | 0 | 0 | 0 |
| 0 | 1 | 1 | 0 |
| 0 | 1 | 0 | 0 |
| 0 | 0 | 1 | 0 |
| 0 | 0 | 0 | 0 |


1. View all the lines  where the output is given.
1. From these construct a formulas with all inputs where the output is satisfied ANDed together.
1. OR all these atoms together.

This will give you:

&#92;[(P\wedge Q \wedge R)\vee(P\wedge\neg Q\wedge R)\vee(P\wedge Q\wedge\neg R)&#92;]

This is the **disjunctive normal form** (DNF).
{:.info}

You can then convert this into a circuit diagram:

![from table]({site.baseurl}/assets/COMP109/Lectures/2020-12-03-1-8.svg)

This formula and diagram can be simplified to give the following:

&#92;[P\wedge (Q\vee R)&#92;]

![from table]({site.baseurl}/assets/COMP109/Lectures/2020-12-03-1-9.svg)

You can see this from investigating the table.

### Circuit Equivalence
Two circuits are equivalent if they produce the same output given the same input.

### Logical Equivalence
Two formulas &#92;(P&#92;) and &#92;(Q&#92;) are called equivalent if they have the same truth value uder every possible interpretation. In other words, &#92;(P&#92;) and &#92;(Q&#92;)Q are equivalent if &#92;(I(p)=I(Q)&#92;) for every interpretation &#92;(I&#92;). This is denoted by:

&#92;[P\equiv Q&#92;]

#### Theorem
The relation &#92;(\equiv&#92;) is an equivalence relation on &#92;(\mathcal{P}&#92;).

#### Proof
* &#92;(\equiv&#92;) is reflexive, since, trivially, &#92;(I(P)=I(P)&#92;) for every interpretation &#92;(I&#92;).
* &#92;(\equiv&#92;) is transitive, since &#92;(P\equiv Q&#92;) and &#92;(Q\equiv R&#92;) implies &#92;(P\equiv R&#92;).
* &#92;(\equiv&#92;) is symmetric, since &#92;(P\equiv Q&#92;) implies &#92;(Q\equiv P&#92;).

### Useful Equivalences
#### Associative Laws
&#92;[
\begin{aligned}
(P\vee (Q\vee R))&\equiv((P\vee Q)\vee R)&#92;&#92;
(P\wedge (Q\wedge R))&\equiv((P\wedge Q)\wedge R)
\end{aligned}
&#92;]

#### Commutative Laws
&#92;[
\begin{aligned}
(P\vee Q)&\equiv (Q\vee P)&#92;&#92;
(P\wedge Q)&\equiv (Q\wedge P)
\end{aligned}
&#92;]

#### Identity Laws
&#92;[
\begin{aligned}
(P\vee\bot)&\equiv P&#92;&#92;
(P\vee\top)&\equiv \top&#92;&#92;
(P\wedge\top)&\equiv P&#92;&#92;
(P\wedge\bot)&\equiv \bot
\end{aligned}
&#92;]

#### Distributive Laws
&#92;[
\begin{aligned}
(P\wedge(Q\vee R))&\equiv((P\wedge Q)\vee(P\wedge R))&#92;&#92;
(P\vee(Q\wedge R))&\equiv((P\vee Q)\wedge(P\vee R))
\end{aligned}
&#92;]

#### Complement Laws
&#92;[
\begin{aligned}
P\vee\neg P&\equiv\top&#92;&#92;
\neg\top&\equiv\bot&#92;&#92;
\neg\neg P&\equiv P&#92;&#92;
P\wedge\neg P&\equiv\bot&#92;&#92;
\neg\bot&\equiv\top
\end{aligned}
&#92;]

#### De Morgan's Laws
&#92;[
\begin{aligned}
\neg(P\vee Q)&\equiv(\neg P\wedge \neg Q)&#92;&#92;
\neg(P\wedge Q)&\equiv(\neg P\vee \neg Q)
\end{aligned}
&#92;]
