---
title: Lecture 9-2
tags: COMP105 Lectures
---
## Recursion with Multiple Lists
Sometimes we want to use recursion on more than one list at a time. The following example adds the elements of two lists together:

```haskell
add_lists _ [] = []
add_lists [] _ = []
addlists (x:xs) (y:ys) = x + y : addlists xs ys
```

* Base cases stop when either of the lists is empty.
* Recursive rule pulls an element form both lists.

Another method to implement this, provided that you don't want to accept lists which don't have equal length is like the following:

```haskell
f [] [] = []
f [] _ = error "Second list is longer"
f _ [] = error "First list is longer"
f (x:xs) (y:ys) = x + y : f xs ys
```

* This will give an explicit error if they aren't matching length.

### Splitting a List in Two
Other functions can take a list and return a pair of lists:

```haskell
gt_10 [] = ([],[])
gt_10 (x:xs)
	| x > 10	= (x:gt, lt)
	| otherwise	= (gt, x:lt)
	where (gt, lt) = gt_10 xs
```

This will split a list into two lists containing values that are bigger and smaller than 10. 

* The base case sets up the tuple.
* The recursive rule modifies one of the two lists. 

### `zip`
`zip` takes two lists and returns a list of pairs

```haskell
zip' [] _ = []
zip' _ [] = []
zip' (x:xs) (y:ys) = (x, y) : zip' xs ys
```

## Exercises
1. ```haskell
	multiplyLists _ [] = []
	multiplyLists [] _ = []
	multiplyLists (x:xs) (y:ys) = x * y : multiplyLists xs ys
	```

1. ```haskell
	zip3' [] _ _ = []
	zip3' _ [] _ = []
	zip3' _ _ [] = []
	zip3' (x:xs) (y:ys) (z:zs) = (x,y,z) : zip3' xs ys zs
	```